Iris/Iris/Tests/WeakestPre.lean
@@ -118,37 +118,6 @@ variable (Φ : Val → PROP)
 
 end TestWP
 
-section TestTotalTexanTriple
-
-set_option linter.unusedVariables false
-
-variable (PROP Expr Val A : Type _) [BI PROP]
-variable [TotalWp PROP Expr Val A] [TotalWp PROP Expr Val Stuckness]
-variable (e : Expr) (s : A) (E : CoPset) (P Q : PROP) (v : Val)
-
-/-- info: iprop(∀ Φ, P -∗ (Q -∗ Φ v) -∗ WP e @ s ; E [{ Φ }] ) : PROP -/
-#guard_msgs in #check [[{ P }]] e @ s ; E [[{ RET v; Q }]]
-
-/-- info: iprop(∀ Φ, P -∗ (Q -∗ Φ v) -∗ WP e @ E [{ Φ }] ) : PROP -/
-#guard_msgs in #check [[{ P }]] e @ E [[{ RET v; Q }]]
-
-/-- info: iprop(∀ Φ, P -∗ (Q -∗ Φ v) -∗ WP e @ E ? [{ Φ }] ) : PROP -/
-#guard_msgs in #check [[{ P }]] e @ E ? [[{ RET v; Q }]]
-
-/-- info: iprop(∀ Φ, P -∗ (Q -∗ Φ v) -∗ WP e [{ Φ }] ) : PROP -/
-#guard_msgs in #check [[{ P }]] e [[{ RET v; Q }]]
-
-/-- info: iprop(∀ Φ, P -∗ (Q -∗ Φ v) -∗ WP e ? [{ Φ }] ) : PROP -/
-#guard_msgs in #check [[{ P }]] e ? [[{ RET v; Q }]]
-
-/-- info: iprop(∀ Φ, P -∗ (∀ x, Q -∗ Φ x) -∗ WP e [{ Φ }] ) : PROP -/
-#guard_msgs in #check [[{ P }]] e [[{ (x : Val), RET x; Q }]]
-
-/-- info: iprop(∀ Φ, P -∗ (∀ x, Q -∗ Φ v) -∗ WP e [{ Φ }] ) : PROP -/
-#guard_msgs in #check [[{ P }]] e [[{ _, RET v; Q }]]
-
-end TestTotalTexanTriple
-
 section TestTexanTriple
 
 set_option linter.unusedVariables false
@@ -222,6 +191,56 @@ variable (P Q : PROP)
 #guard_msgs in #check iprop({{ P }} e ? {{ RET 0 ; Q }})
 
 end TestTexanTriple
+
+section TestTotalTexanTriple
+
+variable (PROP Expr Val A : Type _) [BI PROP]
+variable [TotalWp PROP Expr Val A] [TotalWp PROP Expr Val Stuckness]
+variable (e : Expr) (s : A) (E : CoPset) (P Q : PROP) (v : Val)
+
+/-- info: ⊢ ∀ Φ, P -∗ (Q -∗ Φ v) -∗ WP e @ s ; E [{ Φ }] : Prop -/
+#guard_msgs in #check [{ P }] e @ s ; E [{ RET v; Q }]
+
+/-- info: ⊢ ∀ Φ, P -∗ (Q -∗ Φ v) -∗ WP e @ E [{ Φ }] : Prop -/
+#guard_msgs in #check [{ P }] e @ E [{ RET v; Q }]
+
+/-- info: ⊢ ∀ Φ, P -∗ (Q -∗ Φ v) -∗ WP e @ E ? [{ Φ }] : Prop -/
+#guard_msgs in #check [{ P }] e @ E ? [{ RET v; Q }]
+
+/-- info: ⊢ ∀ Φ, P -∗ (Q -∗ Φ v) -∗ WP e [{ Φ }] : Prop -/
+#guard_msgs in #check [{ P }] e [{ RET v; Q }]
+
+/-- info: ⊢ ∀ Φ, P -∗ (Q -∗ Φ v) -∗ WP e ? [{ Φ }] : Prop -/
+#guard_msgs in #check [{ P }] e ? [{ RET v; Q }]
+
+/-- info: ⊢ ∀ Φ, P -∗ (∀ x, Q -∗ Φ x) -∗ WP e [{ Φ }] : Prop -/
+#guard_msgs in #check [{ P }] e [{ (x : Val), RET x; Q }]
+
+/-- info: ⊢ ∀ Φ, P -∗ (∀ x, Q -∗ Φ v) -∗ WP e [{ Φ }] : Prop -/
+#guard_msgs in #check [{ P }] e [{ _, RET v; Q }]
+
+/-- info: iprop(□ ∀ Φ, P -∗ (Q -∗ Φ v) -∗ WP e @ s ; E [{ Φ }] ) : PROP -/
+#guard_msgs in #check iprop([{ P }] e @ s ; E [{ RET v; Q }])
+
+/-- info: iprop(□ ∀ Φ, P -∗ (Q -∗ Φ v) -∗ WP e @ E [{ Φ }] ) : PROP -/
+#guard_msgs in #check iprop([{ P }] e @ E [{ RET v; Q }])
+
+/-- info: iprop(□ ∀ Φ, P -∗ (Q -∗ Φ v) -∗ WP e @ E ? [{ Φ }] ) : PROP -/
+#guard_msgs in #check iprop([{ P }] e @ E ? [{ RET v; Q }])
+
+/-- info: iprop(□ ∀ Φ, P -∗ (Q -∗ Φ v) -∗ WP e [{ Φ }] ) : PROP -/
+#guard_msgs in #check iprop([{ P }] e [{ RET v; Q }])
+
+/-- info: iprop(□ ∀ Φ, P -∗ (Q -∗ Φ v) -∗ WP e ? [{ Φ }] ) : PROP -/
+#guard_msgs in #check iprop([{ P }] e ? [{ RET v; Q }])
+
+/-- info: iprop(□ ∀ Φ, P -∗ (∀ x, Q -∗ Φ x) -∗ WP e [{ Φ }] ) : PROP -/
+#guard_msgs in #check iprop([{ P }] e [{ (x : Val), RET x; Q }])
+
+/-- info: iprop(□ ∀ Φ, P -∗ (∀ x, Q -∗ Φ v) -∗ WP e [{ Φ }] ) : PROP -/
+#guard_msgs in #check iprop([{ P }] e [{ _, RET v; Q }])
+
+end TestTotalTexanTriple
 
 section HeapLangTestWP
 set_option linter.unusedVariables false
@@ -318,4 +337,3 @@ info: iprop(□ ∀ Φ, P -∗ (▷ ∀ x, Q -∗ Φ x) -∗ WP hl(if (#1 < #2) 
 #guard_msgs in #check iprop({{ P }} hl(#1) {{ v, RET v; ⌜v = hl_val(#1)⌝ }} : PROP)
 
 end HeapLangTestTexanTriple
-
